Locally_Nameless_Lambda_Calculus/LN_Lambda_Typing.thy
@@ -1,31 +1,360 @@
 theory LN_Lambda_Typing
   imports
+    "HOL-Library.Dlist"
     LN_Lambda_Term
+    "Abstract_Substitution.Substitution"
 begin
 
-datatype ('\<alpha>, '\<kappa>) ty =
-  TyVar '\<alpha> |
-  TyCtr '\<kappa> "('\<alpha>, '\<kappa>) ty list" |
-  TyBool |
-  TyFun "('\<alpha>, '\<kappa>) ty" "('\<alpha>, '\<kappa>) ty"
+abbreviation fold2 :: "('a \<Rightarrow> 'b \<Rightarrow> 'c \<Rightarrow> 'c) \<Rightarrow> 'a list \<Rightarrow> 'b list \<Rightarrow> 'c \<Rightarrow> 'c" where
+  "fold2 f xs ys \<equiv> fold (\<lambda>(x, y). f x y) (zip xs ys)"
 
-type_synonym ('\<alpha>, '\<kappa>) const_ty = "'\<alpha> list \<times> ('\<alpha>, '\<kappa>) ty list \<times> ('\<alpha>, '\<kappa>) ty"
+definition fun_upds :: "('a \<Rightarrow> 'b) \<Rightarrow> 'a list \<Rightarrow> 'b list \<Rightarrow> ('a \<Rightarrow> 'b)" where
+  "fun_upds f xs ys = fold2 (\<lambda>x y f. f(x := y)) xs ys f"
+
+class arity =
+  fixes arity :: "'a \<Rightarrow> nat"
+
+class term_signature =
+  fixes
+    True_tconst :: 'a and
+    False_tconst :: 'a and
+    Neg_tconst :: 'a and
+    Conj_tconst :: 'a and
+    Disj_tconst :: 'a and
+    Imp_tconst :: 'a and
+    Eq_tconst :: 'a and
+    Neq_tconst :: 'a
+
+class type_signature = arity +
+  fixes bool_tyctr :: 'a and fun_tyctr :: 'a
+  assumes arity\<^sub>_tyctr_simps[simp]: "arity bool_tyctr = 0" "arity fun_tyctr = 2"
+
+
+section \<open>Pretypes\<close>
+
+datatype (type_vars_prety: '\<V>\<^sub>t\<^sub>y, '\<Sigma>\<^sub>t\<^sub>y) prety =
+  PretyVar '\<V>\<^sub>t\<^sub>y |
+  PretyCtr '\<Sigma>\<^sub>t\<^sub>y "('\<V>\<^sub>t\<^sub>y, '\<Sigma>\<^sub>t\<^sub>y) prety list"
+
+
+subsection \<open>Substitutions\<close>
+
+primrec subst_prety ::
+  "('\<V>\<^sub>t\<^sub>y, '\<Sigma>\<^sub>t\<^sub>y) prety \<Rightarrow> ('\<V>\<^sub>t\<^sub>y \<Rightarrow> ('\<V>\<^sub>t\<^sub>y, '\<Sigma>\<^sub>t\<^sub>y) prety) \<Rightarrow> ('\<V>\<^sub>t\<^sub>y, '\<Sigma>\<^sub>t\<^sub>y) prety" where
+  "subst_prety (PretyVar x) \<sigma> = \<sigma> x" |
+  "subst_prety (PretyCtr \<kappa> \<tau>s) \<sigma> = PretyCtr \<kappa> (map (\<lambda>\<tau>. subst_prety \<tau> \<sigma>) \<tau>s)"
+
+lemma subst_prety_PretyVar[simp]: "subst_prety \<tau> PretyVar = \<tau>"
+proof (induction \<tau>)
+  case (PretyVar x)
+  then show ?case
+    by simp
+next
+  case (PretyCtr \<kappa> \<tau>s)
+  then show ?case
+    by (simp add: list.map_ident_strong)
+qed
+
+definition comp_subst_prety ::
+  "('\<V>\<^sub>t\<^sub>y \<Rightarrow> ('\<V>\<^sub>t\<^sub>y, '\<Sigma>\<^sub>t\<^sub>y) prety) \<Rightarrow> ('\<V>\<^sub>t\<^sub>y \<Rightarrow> ('\<V>\<^sub>t\<^sub>y, '\<Sigma>\<^sub>t\<^sub>y) prety) \<Rightarrow> '\<V>\<^sub>t\<^sub>y \<Rightarrow> ('\<V>\<^sub>t\<^sub>y, '\<Sigma>\<^sub>t\<^sub>y) prety" where
+  "comp_subst_prety \<sigma>\<^sub>1 \<sigma>\<^sub>2 \<equiv> \<lambda>x. subst_prety (\<sigma>\<^sub>1 x) \<sigma>\<^sub>2"
+
+global_interpretation comp_subst_prety: monoid comp_subst_prety PretyVar
+proof unfold_locales
+  fix \<sigma>\<^sub>1 \<sigma>\<^sub>2 \<sigma>\<^sub>3 :: "'\<V>\<^sub>t\<^sub>y \<Rightarrow> ('\<V>\<^sub>t\<^sub>y, '\<Sigma>\<^sub>t\<^sub>y) prety"
+  show "comp_subst_prety (comp_subst_prety \<sigma>\<^sub>1 \<sigma>\<^sub>2) \<sigma>\<^sub>3 = comp_subst_prety \<sigma>\<^sub>1 (comp_subst_prety \<sigma>\<^sub>2 \<sigma>\<^sub>3)"
+    unfolding comp_subst_prety_def
+  proof (intro ext)
+    have "subst_prety (subst_prety t \<sigma>\<^sub>2) \<sigma>\<^sub>3 = subst_prety t (\<lambda>x. subst_prety (\<sigma>\<^sub>2 x) \<sigma>\<^sub>3)" for t
+    proof (induction t)
+      case (PretyVar y)
+      then show ?case
+        by (metis subst_prety.simps(1))
+    next
+      case (PretyCtr \<kappa> \<tau>s)
+      then show ?case
+        unfolding subst_prety.simps prety.inject
+        unfolding list.map_comp comp_def
+        by simp
+    qed
+    then show "\<And>x. subst_prety (subst_prety (\<sigma>\<^sub>1 x) \<sigma>\<^sub>2) \<sigma>\<^sub>3 =
+      subst_prety (\<sigma>\<^sub>1 x) (\<lambda>x. subst_prety (\<sigma>\<^sub>2 x) \<sigma>\<^sub>3)"
+      by metis
+  qed
+next
+  show "\<And>a. comp_subst_prety PretyVar a = a"
+    by (simp add: comp_subst_prety_def)
+next
+  show "\<And>a. comp_subst_prety a PretyVar = a"
+    by (simp add: comp_subst_prety_def)
+qed
+
+global_interpretation subst_prety: substitution where
+  comp_subst = comp_subst_prety and
+  id_subst = PretyVar and
+  subst = subst_prety and
+  is_ground = "\<lambda>\<tau>. type_vars_prety \<tau> = {}"
+proof unfold_locales
+  fix \<tau> :: "('\<V>\<^sub>t\<^sub>y, '\<Sigma>\<^sub>t\<^sub>y) prety" and \<sigma>\<^sub>1 \<sigma>\<^sub>2 :: "'\<V>\<^sub>t\<^sub>y \<Rightarrow> ('\<V>\<^sub>t\<^sub>y, '\<Sigma>\<^sub>t\<^sub>y) prety"
+  show "subst_prety \<tau> (comp_subst_prety \<sigma>\<^sub>1 \<sigma>\<^sub>2) = subst_prety (subst_prety \<tau> \<sigma>\<^sub>1) \<sigma>\<^sub>2"
+    by (induction \<tau>) (simp_all add: comp_subst_prety_def)
+next
+  fix \<tau> :: "('\<V>\<^sub>t\<^sub>y, '\<Sigma>\<^sub>t\<^sub>y) prety"
+  show "subst_prety \<tau> PretyVar = \<tau>"
+    by simp
+next
+  fix \<tau> :: "('\<V>\<^sub>t\<^sub>y, '\<Sigma>\<^sub>t\<^sub>y) prety"
+  assume "type_vars_prety \<tau> = {}"
+  then show "\<forall>\<sigma>. subst_prety \<tau> \<sigma> = \<tau>"
+    by (induction \<tau>) (simp_all add: list.map_ident_strong)
+qed
+                                                            
+section \<open>Well-Formed Types\<close>
+
+inductive wf_prety :: "('\<V>\<^sub>t\<^sub>y, '\<Sigma>\<^sub>t\<^sub>y :: arity) prety \<Rightarrow> bool" where
+  PretyVar: "wf_prety (PretyVar \<alpha>)"
+    for \<alpha> :: '\<V>\<^sub>t\<^sub>y |
+  PretyCtr: "wf_prety (PretyCtr \<kappa> \<tau>s)"
+    if "length \<tau>s = arity \<kappa>" and "\<forall>\<tau> \<in> set \<tau>s. wf_prety \<tau>"
+    for \<kappa> :: '\<Sigma>\<^sub>t\<^sub>y and \<tau>s :: "('\<V>\<^sub>t\<^sub>y, '\<Sigma>\<^sub>t\<^sub>y) prety list"
+
+typedef (overloaded) ('\<V>\<^sub>t\<^sub>y, '\<Sigma>\<^sub>t\<^sub>y :: arity) ty = \<open>{\<tau> :: ('\<V>\<^sub>t\<^sub>y, '\<Sigma>\<^sub>t\<^sub>y) prety. wf_prety \<tau>}\<close>
+  morphisms Rep_ty Abs_ty
+proof
+  show \<open>PretyVar undefined \<in> {\<tau>. wf_prety \<tau>}\<close>
+    by (blast intro: wf_prety.intros)
+qed
+
+setup_lifting type_definition_ty
+
+lift_definition TyVar :: "'\<V>\<^sub>t\<^sub>y \<Rightarrow> ('\<V>\<^sub>t\<^sub>y, '\<Sigma>\<^sub>t\<^sub>y :: arity) ty" is PretyVar
+  by (rule wf_prety.PretyVar)
+
+definition TyCtr :: "'\<Sigma>\<^sub>t\<^sub>y \<Rightarrow> ('\<V>\<^sub>t\<^sub>y, '\<Sigma>\<^sub>t\<^sub>y) ty list \<Rightarrow> ('\<V>\<^sub>t\<^sub>y, '\<Sigma>\<^sub>t\<^sub>y :: arity) ty" where
+  "TyCtr \<kappa> \<tau>s = Abs_ty (PretyCtr \<kappa> (map Rep_ty \<tau>s))"
+
+lemma wf_prety_PretyCtr:
+  assumes "length \<tau>s = arity \<kappa>"
+  shows "wf_prety (PretyCtr \<kappa> (map Rep_ty \<tau>s))"
+proof (rule wf_prety.PretyCtr)
+  show "\<forall>\<tau>\<in>set (map Rep_ty \<tau>s). wf_prety \<tau>"
+    using Rep_ty by auto
+qed (use assms in simp_all)
+
+
+subsection \<open>Injection\<close>
+
+lemma ty_inject[simp]:
+  "TyVar x = TyVar y \<longleftrightarrow> x = y"
+  "length \<tau>s\<^sub>1 = arity \<kappa>\<^sub>1 \<Longrightarrow> length \<tau>s\<^sub>2 = arity \<kappa>\<^sub>2 \<Longrightarrow>
+    TyCtr \<kappa>\<^sub>1 \<tau>s\<^sub>1 = TyCtr \<kappa>\<^sub>2 \<tau>s\<^sub>2 \<longleftrightarrow> \<kappa>\<^sub>1 = \<kappa>\<^sub>2 \<and> \<tau>s\<^sub>1 = \<tau>s\<^sub>2"
+proof -
+  show "TyVar x = TyVar y \<longleftrightarrow> x = y"
+    by (metis TyVar.rep_eq prety.inject(1))
+  show "length \<tau>s\<^sub>1 = arity \<kappa>\<^sub>1 \<Longrightarrow> length \<tau>s\<^sub>2 = arity \<kappa>\<^sub>2 \<Longrightarrow>
+    TyCtr \<kappa>\<^sub>1 \<tau>s\<^sub>1 = TyCtr \<kappa>\<^sub>2 \<tau>s\<^sub>2 \<longleftrightarrow> \<kappa>\<^sub>1 = \<kappa>\<^sub>2 \<and> \<tau>s\<^sub>1 = \<tau>s\<^sub>2"
+    unfolding TyCtr_def
+    by (metis Abs_ty_inject[of "PretyCtr \<kappa>\<^sub>2 (map Rep_ty \<tau>s\<^sub>2)" "PretyCtr \<kappa>\<^sub>1 (map Rep_ty \<tau>s\<^sub>1)"]
+        Rep_ty_inject list.inj_map_strong[of \<tau>s\<^sub>1 \<tau>s\<^sub>2 Rep_ty Rep_ty] mem_Collect_eq prety.inject(2)
+        wf_prety_PretyCtr)
+qed
+
+subsection \<open>Induction and Cases rules\<close>
+
+lemma ty_induct [case_names TyVar TyCtr, induct type: ty]:
+  assumes
+    TyVar_case: "\<And>x. P (TyVar x)" and
+    TyCtr_case: "\<And>\<kappa> \<tau>s. length \<tau>s = arity \<kappa> \<Longrightarrow> (\<And>\<tau>. \<tau> \<in> set \<tau>s \<Longrightarrow> P \<tau>) \<Longrightarrow> P (TyCtr \<kappa> \<tau>s)"
+  shows "P x"
+proof (cases x)
+  case (Abs_ty \<tau>)
+  then have "wf_prety \<tau>"
+    by simp
+  then show ?thesis
+    unfolding \<open>x = Abs_ty \<tau>\<close>
+  proof (induction \<tau>)
+    case (PretyVar y)
+    show ?case
+      unfolding TyVar.abs_eq[symmetric]
+      using TyVar_case .
+  next
+    case (PretyCtr \<kappa> \<tau>s)
+
+    have "P (Abs_ty (PretyCtr \<kappa> (map Rep_ty (map Abs_ty \<tau>s))))"
+    proof (rule TyCtr_case[unfolded TyCtr_def])
+      show "length (map Abs_ty \<tau>s) = arity \<kappa>"
+        by (simp add: PretyCtr.hyps)
+    next
+      show "\<And>\<tau>. \<tau> \<in> set (map Abs_ty \<tau>s) \<Longrightarrow> P \<tau>"
+        using PretyCtr.IH by auto
+    qed
+
+    moreover have "map Rep_ty (map Abs_ty \<tau>s) = \<tau>s"
+      unfolding list.map_comp comp_def
+    proof (rule list.map_ident_strong)
+      show "\<And>z. z \<in> set \<tau>s \<Longrightarrow> Rep_ty (Abs_ty z) = z"
+        by (simp add: Abs_ty_inverse PretyCtr.IH)
+    qed
+
+    ultimately show ?case
+      by metis
+  qed
+qed
+
+lemma ty_exhaust [case_names TyVar TyCtr]:
+  assumes
+    TyVar_case: "\<And>x. \<tau> = TyVar x \<Longrightarrow> thesis" and
+    TyCtr_case: "\<And>\<kappa> \<tau>s. \<tau> = TyCtr \<kappa> \<tau>s \<Longrightarrow> length \<tau>s = arity \<kappa> \<Longrightarrow> thesis"
+  shows thesis
+  using assms
+  by (induction \<tau>) metis+
+
+
+subsection \<open>Type Variables\<close>
+
+lift_definition type_vars :: "('\<V>\<^sub>t\<^sub>y, '\<Sigma>\<^sub>t\<^sub>y :: arity) ty \<Rightarrow> '\<V>\<^sub>t\<^sub>y set"
+  is type_vars_prety .
+
+lemma type_vars_TyVar[simp]: "type_vars (TyVar x) = {x}"
+  by (simp add: TyVar.rep_eq type_vars.rep_eq)
+
+lemma type_vars_TyCtr[simp]:
+  "length \<tau>s = arity \<kappa> \<Longrightarrow> type_vars (TyCtr \<kappa> \<tau>s) = (\<Union>\<tau> \<in> set \<tau>s. type_vars \<tau>)"
+  by (simp add: Abs_ty_inverse TyCtr_def type_vars_def wf_prety_PretyCtr)
+
+
+subsection \<open>Common Types\<close>
+
+lemma wf_prety_PretyCtr_bool_tyctr[intro]: "wf_prety (PretyCtr bool_tyctr [])"
+  by (rule wf_prety.PretyCtr) simp_all
+
+definition TyBool :: "('\<V>\<^sub>t\<^sub>y, '\<Sigma>\<^sub>t\<^sub>y :: type_signature) ty" where
+  "TyBool \<equiv> Abs_ty (PretyCtr bool_tyctr [])"
+
+
+lemma wf_prety_PretyCtr_fun_tyctr[intro]: "wf_prety (PretyCtr fun_tyctr [Rep_ty \<tau>\<^sub>1, Rep_ty \<tau>\<^sub>2])"
+proof (intro wf_prety.PretyCtr[rule_format])
+  show "\<And>x. x \<in> set [Rep_ty \<tau>\<^sub>1, Rep_ty \<tau>\<^sub>2] \<Longrightarrow> wf_prety x"
+    using Rep_ty by auto
+qed simp_all
+
+definition TyFun ::
+  "('\<V>\<^sub>t\<^sub>y, '\<Sigma>\<^sub>t\<^sub>y :: type_signature) ty \<Rightarrow> ('\<V>\<^sub>t\<^sub>y, '\<Sigma>\<^sub>t\<^sub>y :: type_signature) ty \<Rightarrow>
+    ('\<V>\<^sub>t\<^sub>y, '\<Sigma>\<^sub>t\<^sub>y :: type_signature) ty" where
+  "TyFun \<tau>\<^sub>1 \<tau>\<^sub>2 \<equiv> Abs_ty (PretyCtr fun_tyctr [Rep_ty \<tau>\<^sub>1, Rep_ty \<tau>\<^sub>2])"
+
+
+subsection \<open>Substitutions\<close>
+
+lift_definition subst_ty ::
+  "('\<V>\<^sub>t\<^sub>y, '\<Sigma>\<^sub>t\<^sub>y :: arity) ty \<Rightarrow> ('\<V>\<^sub>t\<^sub>y \<Rightarrow> ('\<V>\<^sub>t\<^sub>y, '\<Sigma>\<^sub>t\<^sub>y) ty) \<Rightarrow> ('\<V>\<^sub>t\<^sub>y, '\<Sigma>\<^sub>t\<^sub>y) ty" (infix "\<cdot>\<^sub>t\<^sub>y" 55)
+  is subst_prety
+proof -
+  fix \<tau> :: "('\<V>\<^sub>t\<^sub>y, '\<Sigma>\<^sub>t\<^sub>y) prety" and \<sigma> :: "'\<V>\<^sub>t\<^sub>y \<Rightarrow> ('\<V>\<^sub>t\<^sub>y, '\<Sigma>\<^sub>t\<^sub>y) prety"
+  assume "wf_prety \<tau>" and "\<And>x. wf_prety (\<sigma> x)"
+  then show "wf_prety (subst_prety \<tau> \<sigma>)"
+    by (induction \<tau> rule: wf_prety.induct) (simp_all add: wf_prety.PretyCtr)
+qed
+
+lemma subst_ty_simps[simp]:
+  "TyVar x \<cdot>\<^sub>t\<^sub>y \<sigma> = \<sigma> x"
+  "length \<tau>s = arity \<kappa> \<Longrightarrow> TyCtr \<kappa> \<tau>s \<cdot>\<^sub>t\<^sub>y \<sigma> = TyCtr \<kappa> (map (\<lambda>\<tau>. \<tau> \<cdot>\<^sub>t\<^sub>y \<sigma>) \<tau>s)"
+proof -
+  show "TyVar x \<cdot>\<^sub>t\<^sub>y \<sigma> = \<sigma> x"
+    by (metis Rep_ty_inject TyVar.rep_eq comp_def id_apply subst_prety.simps(1) subst_ty.rep_eq)
+  show "length \<tau>s = arity \<kappa> \<Longrightarrow> TyCtr \<kappa> \<tau>s \<cdot>\<^sub>t\<^sub>y \<sigma> = TyCtr \<kappa> (map (\<lambda>\<tau>. \<tau> \<cdot>\<^sub>t\<^sub>y \<sigma>) \<tau>s)"
+    by (smt (verit, best) Abs_ty_inverse Rep_ty_inverse
+        TyCtr_def list.map_comp map_eq_conv
+        mem_Collect_eq o_def subst_prety.simps(2)
+        subst_ty.rep_eq wf_prety_PretyCtr)
+qed
+
+lemma subst_ty_TyVar[simp]: "\<tau> \<cdot>\<^sub>t\<^sub>y TyVar = \<tau>"
+  by (induction \<tau> rule: ty_induct) (simp_all add: list.map_ident_strong)
+
+lift_definition comp_subst_ty ::
+  "('\<V>\<^sub>t\<^sub>y \<Rightarrow> ('\<V>\<^sub>t\<^sub>y, '\<Sigma>\<^sub>t\<^sub>y) ty) \<Rightarrow> ('\<V>\<^sub>t\<^sub>y \<Rightarrow> ('\<V>\<^sub>t\<^sub>y, '\<Sigma>\<^sub>t\<^sub>y) ty) \<Rightarrow> '\<V>\<^sub>t\<^sub>y \<Rightarrow> ('\<V>\<^sub>t\<^sub>y, '\<Sigma>\<^sub>t\<^sub>y :: arity) ty"
+  (infix "\<circ>\<^sub>t\<^sub>y" 50) is comp_subst_prety
+  by (metis (no_types, lifting) rel_fun_eq_rel[of "eq_onp wf_prety"] eq_onp_same_args[of wf_prety]
+      subst_ty.rsp
+      rel_funD2[of "rel_fun (=) (eq_onp wf_prety)" "eq_onp wf_prety" "subst_prety _"
+        "subst_prety _"]
+      rel_funD2[of "eq_onp wf_prety" "rel_fun (rel_fun (=) (eq_onp wf_prety)) (eq_onp wf_prety)"
+        subst_prety subst_prety]
+      comp_subst_prety_def)
+
+lemma comp_subst_ty_conv: "\<sigma>\<^sub>1 \<circ>\<^sub>t\<^sub>y \<sigma>\<^sub>2 = (\<lambda>x. \<sigma>\<^sub>1 x \<cdot>\<^sub>t\<^sub>y \<sigma>\<^sub>2)"
+  by (metis (mono_tags, opaque_lifting)
+      Rep_ty_inverse
+      subst_ty.rep_eq[of "\<sigma>\<^sub>1 _" \<sigma>\<^sub>2]
+      comp_subst_ty.rep_eq[of \<sigma>\<^sub>1 \<sigma>\<^sub>2]
+      comp_id[of "Rep_ty \<circ> _"]
+      comp_apply[of Rep_ty]
+      comp_subst_prety_def[of "Rep_ty \<circ> \<sigma>\<^sub>1" "Rep_ty \<circ> \<sigma>\<^sub>2"])
+
+global_interpretation comp_subst_ty: monoid comp_subst_ty TyVar
+proof unfold_locales
+  fix \<sigma>\<^sub>1 \<sigma>\<^sub>2 \<sigma>\<^sub>3 :: "'\<V>\<^sub>t\<^sub>y \<Rightarrow> ('\<V>\<^sub>t\<^sub>y, '\<Sigma>\<^sub>t\<^sub>y :: arity) ty"
+  show "((\<sigma>\<^sub>1 \<circ>\<^sub>t\<^sub>y \<sigma>\<^sub>2) \<circ>\<^sub>t\<^sub>y \<sigma>\<^sub>3) = (\<sigma>\<^sub>1 \<circ>\<^sub>t\<^sub>y (\<sigma>\<^sub>2 \<circ>\<^sub>t\<^sub>y \<sigma>\<^sub>3))"
+    unfolding comp_subst_ty_conv
+  proof (intro ext)
+    have "(t \<cdot>\<^sub>t\<^sub>y \<sigma>\<^sub>2) \<cdot>\<^sub>t\<^sub>y \<sigma>\<^sub>3 = t \<cdot>\<^sub>t\<^sub>y (\<lambda>x. \<sigma>\<^sub>2 x \<cdot>\<^sub>t\<^sub>y \<sigma>\<^sub>3)" for t
+      by (induction t) simp_all
+
+    then show "\<And>x. (\<sigma>\<^sub>1 x \<cdot>\<^sub>t\<^sub>y \<sigma>\<^sub>2) \<cdot>\<^sub>t\<^sub>y \<sigma>\<^sub>3 = \<sigma>\<^sub>1 x \<cdot>\<^sub>t\<^sub>y (\<lambda>x. \<sigma>\<^sub>2 x \<cdot>\<^sub>t\<^sub>y \<sigma>\<^sub>3)"
+      by metis
+  qed
+next
+  show "\<And>a. (TyVar \<circ>\<^sub>t\<^sub>y a) = a"
+    by (simp add: comp_subst_ty_conv)
+next
+  show "\<And>a. (a \<circ>\<^sub>t\<^sub>y TyVar) = a"
+    by (simp add: comp_subst_ty_conv)
+qed
+
+
+global_interpretation subst_ty: substitution where
+  comp_subst = comp_subst_ty and
+  id_subst = TyVar and
+  subst = subst_ty and
+  is_ground = "\<lambda>\<tau>. type_vars \<tau> = {}"
+proof unfold_locales
+  fix \<tau> :: "('\<V>\<^sub>t\<^sub>y, '\<Sigma>\<^sub>t\<^sub>y :: arity) ty" and \<sigma>\<^sub>1 \<sigma>\<^sub>2 :: "'\<V>\<^sub>t\<^sub>y \<Rightarrow> ('\<V>\<^sub>t\<^sub>y, '\<Sigma>\<^sub>t\<^sub>y) ty"
+  show "\<tau> \<cdot>\<^sub>t\<^sub>y (\<sigma>\<^sub>1 \<circ>\<^sub>t\<^sub>y \<sigma>\<^sub>2) = (\<tau> \<cdot>\<^sub>t\<^sub>y \<sigma>\<^sub>1) \<cdot>\<^sub>t\<^sub>y \<sigma>\<^sub>2"
+    by (induction \<tau>) (simp_all add: comp_subst_ty_conv)
+next
+  fix \<tau> :: "('\<V>\<^sub>t\<^sub>y, '\<Sigma>\<^sub>t\<^sub>y :: arity) ty"
+  show "subst_ty \<tau> TyVar = \<tau>"
+    by simp
+next
+  fix \<tau> :: "('\<V>\<^sub>t\<^sub>y, '\<Sigma>\<^sub>t\<^sub>y :: arity) ty"
+  assume "type_vars \<tau> = {}"
+  then show "\<forall>\<sigma>. \<tau> \<cdot>\<^sub>t\<^sub>y \<sigma> = \<tau>"
+    by (induction \<tau>) (simp_all add: list.map_ident_strong)
+qed
+
+section \<open>Type System\<close>
+
+type_synonym ('\<V>\<^sub>t\<^sub>y, '\<Sigma>\<^sub>t\<^sub>y) const_ty = "'\<V>\<^sub>t\<^sub>y dlist \<times> ('\<V>\<^sub>t\<^sub>y, '\<Sigma>\<^sub>t\<^sub>y) ty list \<times> ('\<V>\<^sub>t\<^sub>y, '\<Sigma>\<^sub>t\<^sub>y) ty"
 
 inductive has_type ::
-  "('c \<rightharpoonup> ('\<alpha>, '\<kappa>) const_ty) \<Rightarrow> ('f \<rightharpoonup> ('\<alpha>, '\<kappa>) ty) \<Rightarrow>
-    (('\<alpha>, '\<kappa>) ty, 'c, 'f) preterm \<Rightarrow> ('\<alpha>, '\<kappa>) ty \<Rightarrow> bool"
+  "('\<Sigma> \<Rightarrow> ('\<V>\<^sub>t\<^sub>y, '\<Sigma>\<^sub>t\<^sub>y :: type_signature) const_ty) \<Rightarrow> ('\<V> \<Rightarrow> ('\<V>\<^sub>t\<^sub>y, '\<Sigma>\<^sub>t\<^sub>y) ty) \<Rightarrow>
+    (('\<V>\<^sub>t\<^sub>y, '\<Sigma>\<^sub>t\<^sub>y) ty, '\<Sigma>, '\<V>) preterm \<Rightarrow> ('\<V>\<^sub>t\<^sub>y, '\<Sigma>\<^sub>t\<^sub>y) ty \<Rightarrow> bool"
   for \<C> where
-  Const: "has_type \<C> \<F> (Const c \<tau>\<^sub>1s ts) \<tau>\<^sub>3"
-    if "\<C> c = Some (\<alpha>s, \<tau>\<^sub>2s, \<tau>\<^sub>3)" and "length \<tau>\<^sub>1s = length \<alpha>s" and "list_all2 (has_type \<C> \<F>) ts \<tau>\<^sub>2s"
-    for \<F> c \<tau>\<^sub>1s ts \<tau>\<^sub>3 |
+  Const: "has_type \<C> \<F> (Const c \<tau>\<^sub>1s ts) \<tau>"
+    if "\<C> c = (\<alpha>s, \<tau>\<^sub>2s, \<tau>\<^sub>3)" and "Dlist.length \<alpha>s = length \<tau>\<^sub>1s" and
+      "\<sigma> = fun_upds TyVar (list_of_dlist \<alpha>s) \<tau>\<^sub>1s" and
+      "list_all2 (has_type \<C> \<F>) ts (map (\<lambda>\<tau>\<^sub>2. \<tau>\<^sub>2 \<cdot>\<^sub>t\<^sub>y \<sigma>) \<tau>\<^sub>2s)" and
+      "\<tau> = \<tau>\<^sub>3 \<cdot>\<^sub>t\<^sub>y \<sigma>"
+    for \<F> :: "'\<Sigma> \<Rightarrow> ('\<V>\<^sub>t\<^sub>y, '\<Sigma>\<^sub>t\<^sub>y :: type_signature) const_ty" and c \<tau>\<^sub>1s ts \<tau> |
   Free: "has_type \<C> \<F> (Free f) \<tau>"
-    if "\<F> f = Some \<tau>"
+    if "\<F> f = \<tau>"
     for \<F> f \<tau> |
   App: "has_type \<C> \<F> (App t\<^sub>1 t\<^sub>2) \<tau>\<^sub>2"
-    if "has_type \<C> \<F> t\<^sub>1 (Fun \<tau>\<^sub>1 \<tau>\<^sub>2)" and "has_type \<C> \<F> t\<^sub>2 \<tau>\<^sub>1"
+    if "has_type \<C> \<F> t\<^sub>1 (TyFun \<tau>\<^sub>1 \<tau>\<^sub>2)" and "has_type \<C> \<F> t\<^sub>2 \<tau>\<^sub>1"
     for \<F> t\<^sub>1 t\<^sub>2 \<tau>\<^sub>1 \<tau>\<^sub>2 |
   Abs: "has_type \<C> \<F> (Abs \<tau>\<^sub>1 t) (TyFun \<tau>\<^sub>1 \<tau>\<^sub>2)"
-    if "\<And>x. x |\<notin>| \<X> \<Longrightarrow> has_type \<C> (\<F>(x \<mapsto> \<tau>\<^sub>1)) (subst_bound 0 (Free x) t) \<tau>\<^sub>2"
+    if "\<And>x. x |\<notin>| \<X> \<Longrightarrow> has_type \<C> (\<F>(x := \<tau>\<^sub>1)) (subst_bound 0 (Free x) t) \<tau>\<^sub>2"
     for \<F> t \<tau>\<^sub>1 \<tau>\<^sub>2 \<X>
 
 lemma locally_closed_if_has_type[intro]: "has_type \<C> \<F> t \<tau> \<Longrightarrow> locally_closed t"
@@ -39,16 +368,22 @@ proof (induction \<F> t \<tau> rule: has_type.induct)
   qed
 qed (auto intro: locally_closed.intros)
 
+lemma free_vars_subst_bound_subset: "free_vars (subst_bound n u t) \<subseteq> free_vars t \<union> free_vars u"
+  by (induction t arbitrary: n) auto
 
-lemma has_type_weaken_funenv: "has_type \<C> \<F> t \<tau>\<^sub>1 \<Longrightarrow> x \<notin> dom \<F> \<Longrightarrow> has_type \<C> (\<F>(x \<mapsto> \<tau>\<^sub>2)) t \<tau>\<^sub>1"
+lemma has_type_weaken_funenv:
+  "has_type \<C> \<F> t \<tau>\<^sub>1 \<Longrightarrow> x \<notin> free_vars t \<Longrightarrow> has_type \<C> (\<F>(x := \<tau>\<^sub>2)) t \<tau>\<^sub>1"
 proof (induction \<F> t \<tau>\<^sub>1 rule: has_type.induct)
-  case (Const \<F> c \<tau>\<^sub>1s ts \<tau>\<^sub>3 \<alpha>s \<tau>\<^sub>2s)
-  then show ?case
-    by (simp add: has_type.Const list_all2_mono)
+  case (Const \<F> c \<tau>\<^sub>1s ts \<tau> \<alpha>s \<tau>\<^sub>2s \<tau>\<^sub>3 \<sigma>)
+  show ?case
+  proof (rule has_type.Const)
+    show "list_all2 (has_type \<C> (\<F>(x := \<tau>\<^sub>2))) ts (map (\<lambda>\<tau>\<^sub>2. \<tau>\<^sub>2 \<cdot>\<^sub>t\<^sub>y \<sigma>) \<tau>\<^sub>2s)"
+      by (rule list.rel_mono_strong[OF Const.IH]) (use Const.prems in force)
+  qed (use Const in simp_all)
 next
   case (Free \<F> f \<tau>)
   then show ?case
-    by (metis Free.prems Free.hyps fun_upd_apply has_type.Free domI)
+    by (simp add: has_type.Free)
 next
   case (App \<F> t\<^sub>1 t\<^sub>2 \<tau>\<^sub>1 \<tau>\<^sub>2)
   then show ?case
@@ -59,11 +394,11 @@ next
   proof (rule has_type.Abs)
     fix y
     assume "y |\<notin>| \<X>"
-    show "has_type \<C> (\<F>(x \<mapsto> \<tau>\<^sub>2, y \<mapsto> \<tau>\<^sub>1)) (subst_bound 0 (Free y) t) \<tau>\<^sub>3"
+    show "has_type \<C> (\<F>(x := \<tau>\<^sub>2, y := \<tau>\<^sub>1)) (subst_bound 0 (Free y) t) \<tau>\<^sub>3"
     proof (cases "x = y")
       case True
 
-      then have "\<F>(x \<mapsto> \<tau>\<^sub>2, y \<mapsto> \<tau>\<^sub>1) = \<F>(y \<mapsto> \<tau>\<^sub>1)"
+      then have "\<F>(x := \<tau>\<^sub>2, y := \<tau>\<^sub>1) = \<F>(y := \<tau>\<^sub>1)"
         by simp
 
       then show ?thesis
@@ -71,24 +406,25 @@ next
     next
       case False
 
-      then have "\<F>(x \<mapsto> \<tau>\<^sub>2, y \<mapsto> \<tau>\<^sub>1) = \<F>(y \<mapsto> \<tau>\<^sub>1, x \<mapsto> \<tau>\<^sub>2)"
+      then have "\<F>(x := \<tau>\<^sub>2, y := \<tau>\<^sub>1) = \<F>(y := \<tau>\<^sub>1, x := \<tau>\<^sub>2)"
         by auto
 
-      moreover have "x \<notin> dom (\<F>(y \<mapsto> \<tau>\<^sub>1))"
-        using \<open>x \<notin> dom \<F>\<close> \<open>x \<noteq> y\<close> by simp
+      moreover have "x \<notin> free_vars (subst_bound 0 (Free y) t)"
+        using \<open>x \<notin> free_vars (Abs \<tau>\<^sub>1 t)\<close>[simplified] \<open>x \<noteq> y\<close>
+        using free_vars_subst_bound_subset by force
 
       ultimately show ?thesis
-        using Abs.IH \<open>y |\<notin>| \<X>\<close> by metis
+        using Abs.IH[OF \<open>y |\<notin>| \<X>\<close>] by metis
     qed
   qed
 qed
 
 lemma has_type_subst_free:
-  fixes t :: "(('\<alpha>, '\<kappa>) ty, 'c, 'f) preterm"
-  assumes inf_vars: "infinite (UNIV :: 'f set)"
-  assumes "has_type \<C> \<F> t \<tau>\<^sub>1" and "finite (dom \<F>)" and "\<F> x = Some \<tau>\<^sub>2" and "has_type \<C> \<F> u \<tau>\<^sub>2"
+  fixes t :: "(('\<V>\<^sub>t\<^sub>y, '\<Sigma>\<^sub>t\<^sub>y :: type_signature) ty, '\<Sigma>\<^sub>t\<^sub>y, '\<V>\<^sub>t\<^sub>y) preterm"
+  assumes inf_vars: "infinite (UNIV :: '\<V>\<^sub>t\<^sub>y set)"
+  assumes "has_type \<C> \<F> t \<tau>\<^sub>1" and "\<F> x = \<tau>\<^sub>2" and "has_type \<C> \<F> u \<tau>\<^sub>2"
   shows "has_type \<C> \<F> (subst_free x u t) \<tau>\<^sub>1"
-  using assms(2-5)
+  using assms(2-4)
 proof (induction \<F> t \<tau>\<^sub>1 rule: has_type.induct)
   case (Const \<F> c \<tau>\<^sub>1s ts \<tau>\<^sub>3 \<alpha>s \<tau>\<^sub>2s)
   then show ?case
@@ -107,38 +443,34 @@ next
     unfolding subst_free.simps
   proof (rule has_type.Abs)
     fix y
-    assume y_in: "y |\<notin>| \<X> |\<union>| Abs_fset (dom \<F>)"
+    assume y_in: "y |\<notin>| finsert x (Abs_fset (free_vars t \<union> free_vars u) |\<union>| \<X>)"
 
-    moreover have "x \<in> dom \<F>"
-      using Abs.prems by auto
-
-    ultimately have "x \<noteq> y"
-      using Abs.prems(1) Abs_fset_inverse by blast
+    then have "x \<noteq> y"
+      by blast
 
     moreover have "locally_closed u"
       using Abs.prems by auto
 
-    moreover have "has_type \<C> (\<F>(y \<mapsto> \<tau>\<^sub>1)) (subst_free x u (subst_bound 0 (Free y) t)) \<tau>\<^sub>3"
+    moreover have "has_type \<C> (\<F>(y := \<tau>\<^sub>1)) (subst_free x u (subst_bound 0 (Free y) t)) \<tau>\<^sub>3"
     proof (rule Abs.IH)
       show "y |\<notin>| \<X>"
         using y_in by simp
     next
-      show "finite (dom (\<F>(y \<mapsto> \<tau>\<^sub>1)))"
-        using Abs.prems by simp
-    next
-      show "(\<F>(y \<mapsto> \<tau>\<^sub>1)) x = Some \<tau>\<^sub>2"
+      show "(\<F>(y := \<tau>\<^sub>1)) x = \<tau>\<^sub>2"
         using Abs.prems \<open>x \<noteq> y\<close> by simp
     next
-      have "y \<notin> dom \<F>"
-        using y_in Abs.prems(1) Abs_fset_inverse by auto
+      have "y \<notin> free_vars u"
+        by (metis y_in finite_vars_term mem_Collect_eq finsertCI finite_Un Abs_fset_inverse Un_iff
+            funionI1)
 
-      then show "has_type \<C> (\<F>(y \<mapsto> \<tau>\<^sub>1)) u \<tau>\<^sub>2"
+      then show "has_type \<C> (\<F>(y := \<tau>\<^sub>1)) u \<tau>\<^sub>2"
         using Abs.prems has_type_weaken_funenv by metis
     qed
 
-    ultimately show "has_type \<C> (\<F>(y \<mapsto> \<tau>\<^sub>1)) (subst_bound 0 (Free y) (subst_free x u t)) \<tau>\<^sub>3"
+    ultimately show "has_type \<C> (\<F>(y := \<tau>\<^sub>1)) (subst_bound 0 (Free y) (subst_free x u t)) \<tau>\<^sub>3"
       using subst_free_commutes_with_subst_bound_Free[OF inf_vars] by metis
   qed
 qed
+
 
 end
